Show any sup is a constant map to a quad term of variables in NoSup
This was surprisingly hard! The trick turns out to be to keep proper
track of the height of terms and say something like "hey, if the
supremum were to give something other than a variable, we'd be too
tall".

Terms/NoSup.v
@@ -1,6 +1,7 @@
-Require Top.Terms.Term.
-Require Top.Terms.Generality.
+Require Import Top.Terms.Term.
+Require Import Top.Terms.Generality.
 Require Import Top.Terms.Perm.
+Require Import Top.Terms.VecUtils.
 Require Import Top.FinSet.FinMod.
 Require Import Top.FinSet.FinSet.
 
@@ -40,25 +41,14 @@ Proof.
   intros v v'; destruct v, v'; (auto || (right; discriminate)).
 Qed.
 
-(** Rather than suffixing everything with [V F a], we import
-    [Term.Term] qualified and then define local things with the right
-    names, specialised to our setup. *)
-
-Definition L := Term.LType V F (Term.Lmodule.Mixin _ _ a).
-
-Definition T := Term.Term L.
-Definition funTerm := Term.funTerm L.
-Definition varTerm := Term.varTerm L.
-Definition subst_endo := Term.subst_endo L.
-Definition Subst := Generality.Subst L.
-Definition smg := Generality.smg L.
+Definition L := LType V F (Lmodule.Mixin _ _ a).
 
 (** Constructing terms with vectors is a little cumbersome. [mkF] is a
     helper for applying the binary operation [Ff]. As you'd hope,
     [mkF] is injective. *)
 
-Definition mkF (t0 t1 : T) : T :=
-  funTerm Ff (VectorDef.cons _ t0 1 (VectorDef.cons _ t1 O (VectorDef.nil _))).
+Definition mkF (t0 t1 : Term L) : Term L :=
+  funTerm L Ff (VectorDef.cons _ t0 1 (VectorDef.cons _ t1 O (VectorDef.nil _))).
 
 Lemma mkF_inj {s0 t0 s1 t1} : mkF s0 s1 = mkF t0 t1 -> s0 = t0 /\ s1 = t1.
 Proof.
@@ -69,7 +59,7 @@ Qed.
    variables. Of course, this is just [varTerm]. This is also
    injective. *)
 
-Definition mkV : V -> T := varTerm.
+Definition mkV : V -> Term L := varTerm L.
 
 Lemma mkV_inj {v v'} : mkV v = mkV v' -> v = v'.
 Proof.
@@ -80,12 +70,12 @@ Qed.
     acts as a homomorphism as you'd hope. *)
 
 Lemma subst_endo_mkF s t0 t1
-  : subst_endo s (mkF t0 t1) = mkF (subst_endo s t0) (subst_endo s t1).
+  : subst_endo L s (mkF t0 t1) = mkF (subst_endo L s t0) (subst_endo L s t1).
 Proof.
   exact eq_refl.
 Qed.
 
-Lemma subst_endo_mkV s v : subst_endo s (mkV v) = s v.
+Lemma subst_endo_mkV s v : subst_endo L s (mkV v) = s v.
 Proof.
   exact eq_refl.
 Qed.
@@ -95,9 +85,9 @@ Qed.
     Eder considers two specially chosen substitutions: [sigma] and
     [tau]. *)
 
-Definition sigma : Subst := fun v => mkF (mkV Vx) (mkF (mkV Vy) (mkV Vz)).
+Definition sigma : Subst L := fun v => mkF (mkV Vx) (mkF (mkV Vy) (mkV Vz)).
 
-Definition tau : Subst := fun v => mkF (mkF (mkV Vx) (mkV Vy)) (mkV Vz).
+Definition tau : Subst L := fun v => mkF (mkF (mkV Vx) (mkV Vy)) (mkV Vz).
 
 (** In Eder's paper, he talks about the set containing [sigma] and
     [tau]. We define sets of substitutions implicitly using predicates
@@ -108,22 +98,22 @@ Definition tau : Subst := fun v => mkF (mkF (mkV Vx) (mkV Vy)) (mkV Vz).
     upper bound over [in_st]. (There are two elements in the set, so
     it's pretty easy to see what you have to do!) *)
 
-Definition in_st (s : Subst) : Prop := s = sigma \/ s = tau.
+Definition in_st (s : Subst L) : Prop := s = sigma \/ s = tau.
 
 Lemma ub_st_elim {rho}
-  : Generality.subst_ub L in_st rho ->
-    smg sigma rho /\ smg tau rho.
+  : subst_ub L in_st rho ->
+    smg L sigma rho /\ smg L tau rho.
 Proof.
-  unfold Generality.subst_ub, in_st, smg; auto.
+  unfold subst_ub, in_st, smg; auto.
 Qed.
 
 Lemma ub_st_intro {rho}
-  : smg sigma rho ->
-    smg tau rho ->
-    Generality.subst_ub L in_st rho.
+  : smg L sigma rho ->
+    smg L tau rho ->
+    subst_ub L in_st rho.
 Proof.
   intros.
-  unfold Generality.subst_ub, in_st; fold smg.
+  unfold subst_ub, in_st; fold smg.
   intro t; destruct 1; congruence.
 Qed.
 
@@ -138,8 +128,8 @@ Qed.
 
 Section sigma_decomp.
   Variable v : V.
-  Variable sigma' rho : Subst.
-  Hypothesis decompH : Term.comp_subst sigma' sigma v = rho v.
+  Variable sigma' rho : Subst L.
+  Hypothesis decompH : comp_subst sigma' sigma v = rho v.
 
   Local Definition s12 := sigma' Vx.
   Local Definition s3 := sigma' Vy.
@@ -156,8 +146,8 @@ End sigma_decomp.
 
 Section tau_decomp.
   Variable v : V.
-  Variable tau' rho : Subst.
-  Hypothesis decompH : Term.comp_subst tau' tau v = rho v.
+  Variable tau' rho : Subst L.
+  Hypothesis decompH : comp_subst tau' tau v = rho v.
 
   Local Definition s1 := tau' Vx.
   Local Definition s2 := tau' Vy.
@@ -169,34 +159,35 @@ Section tau_decomp.
   Qed.
 End tau_decomp.
 
-(** * Quads
+(** * Upper bounds for [in_st]
 
     In what follows, we often want to say "there exist four terms such
     that...". This is a bit unwieldy with four layers of existential
     quantifier, so we define a [Quad] type to hold them.
 
+    We're going to need a variation on the quad type in a minute, so
+    we include an map from the entries to terms. A quad containing
+    terms is a [Quad id].
+
  *)
 
-Inductive Quad := mkQuad { q_t0 : T ; q_t1 : T ; q_t2 : T ; q_t3 : T }.
+Inductive Quad {A : Type} (f : A -> Term L) :=
+  mkQuad { q_t0 : A ; q_t1 : A ; q_t2 : A ; q_t3 : A }.
 
 (** The quad composes to make the term [F (F a b) (F c d)], where [a,
     b, c, d] are the coordinates of the quad. *)
 
-Definition quad_term (q : Quad) : T :=
-  match q with mkQuad t0 t1 t2 t3 => mkF (mkF t0 t1) (mkF t2 t3) end.
-
-(** This is just a helper method for defining functions on [V] by
-    cases. *)
-
-Definition vfun {A : Type} (ax ay az : A) (v : V) : A :=
-  match v with Vx => ax | Vy => ay | Vz => az end.
+Definition quad_term {A : Type} {f : A -> Term L} (q : Quad f) : Term L :=
+  match q with
+    mkQuad _ _ a0 a1 a2 a3 => mkF (mkF (f a0) (f a1)) (mkF (f a2) (f a3))
+  end.
 
 (** If a substitution decomposes with [sigma] and [tau], we can
     actually write down its form explicitly. *)
 
 Lemma subst_is_quad_term {v sigma' tau' rho}
-  : Term.comp_subst sigma' sigma v = rho v ->
-    Term.comp_subst tau' tau v = rho v ->
+  : comp_subst sigma' sigma v = rho v ->
+    comp_subst tau' tau v = rho v ->
     rho v = mkF (mkF (s1 tau') (s2 tau')) (mkF (s3 sigma') (s4 sigma')).
 Proof.
   intros sigmaH tauH.
@@ -208,107 +199,171 @@ Proof.
   congruence.
 Qed.
 
-(** Now we pack [subst_is_quad_term] up into a nicer lemma *)
+(** Now we can pack [subst_is_quad_term] up into a nicer lemma, which
+    shows that every upper bound for [in_st] is a [quad_term]. *)
 
 Lemma form_if_ub {rho}
-  : Generality.subst_ub L in_st rho ->
-    exists q : Quad, forall v, rho v = quad_term q.
+  : subst_ub L in_st rho ->
+    exists q : Quad id, forall v, rho v = quad_term q.
 Proof.
   intro ubH.
   destruct (ub_st_elim ubH) as [ smgsH smgtH ].
   destruct smgsH as [ sigma' sigmaH ].
   destruct smgtH as [ tau' tauH ].
-  exists (mkQuad (s1 tau') (s2 tau') (s3 sigma') (s4 sigma')).
+  exists (mkQuad _ _ (s1 tau') (s2 tau') (s3 sigma') (s4 sigma')).
   intro v; unfold quad_term.
   apply subst_is_quad_term; auto.
 Qed.
 
-(*
+(** The converse is also true: every [quad_term] is an upper bound for
+    [in_st]. To make the definition slick, we define [vfun], a helper
+    method for defining functions on [V] by cases. *)
 
-Lemma ub_if_form {q} rho : (forall v, rho v = quad_term q) -> subst_ub
-  V F a in_st rho.  Proof.  intro formH.  destruct q as [ t0 t1 t2 t3
-  ].  intro t; destruct 1 as [ -> | -> ].  - exists (vfun (mkF t0 t1)
-  t2 t3); intro v; destruct v; unfold vfun, comp_subst, compose;
-  simpl; fold (mkF t2 t3); fold (mkF (mkF t0 t1) (mkF t2 t3)); auto.
-  - exists (vfun t0 t1 (mkF t2 t3)); intro v; destruct v; unfold vfun,
-  comp_subst, compose; simpl; fold (mkF t0 t1); fold (mkF (mkF t0 t1)
-  (mkF t2 t3)); auto.  Qed.
+Definition vfun {A : Type} (ax ay az : A) (v : V) : A :=
+  match v with Vx => ax | Vy => ay | Vz => az end.
 
-(** We want to show that if [rho] is a supremum for [in_st] then in
-    any quad form for [rho], each [t0] through [t3] is of the form
-    [mkV v0] through [mkV v3].  *) Inductive VQuad := mkVQuad { v_t0 :
-    V ; v_t1 : V ; v_t2 : V ; v_t3 : V }.
+Lemma ub_if_form {q : Quad id} rho
+  : (forall v, rho v = quad_term q) -> Generality.subst_ub L in_st rho.
+Proof.
+  destruct q as [ t0 t1 t2 t3 ].
+  intros formH; apply ub_st_intro;
+    [ exists (vfun (mkF t0 t1) t2 t3) | exists (vfun t0 t1 (mkF t2 t3)) ];
+    intro v; destruct v; auto.
+Qed.
 
-Definition vquad_to_quad (vq : VQuad) : Quad := mkQuad (mkV (v_t0 vq))
-  (mkV (v_t1 vq)) (mkV (v_t2 vq)) (mkV (v_t3 vq)).
+(** * Supremums for [in_st]
 
-Lemma factor_var_map {v q sigma rho vq} : (rho v = quad_term q) ->
-  (comp_subst sigma rho v = quad_term (vquad_to_quad vq)) -> exists
-  vq', rho v = quad_term (vquad_to_quad vq').  Proof.  intros rhoH H.
-  unfold comp_subst, compose in H.  unfold subst_endo at 2 in H.
-  destruct q as [ t0 t1 t2 t3 ].  rewrite rhoH in *; clear rhoH.
-  simpl in H; simpl.  injection H; clear H; intros H3 H2 H1 H0.
-  destruct vq as [ v0 v1 v2 v3 ]; simpl in *.  (* Each Hi implies ti
-  is a variable *) repeat match goal with | [ H : subst_endo V F a
-  sigma ?t = mkV ?v |- _ ] => let H' := fresh in rename H into H';
-  assert (exists w, t = varTerm V F a w) as H; try solve [(destruct t
-  as [ w | ]; (exists w; auto) || inversion H')]; clear H' end.
-  destruct H0 as [ w0 H0 ].  destruct H1 as [ w1 H1 ].  destruct H2 as
-  [ w2 H2 ].  destruct H3 as [ w3 H3 ].  exists (mkVQuad w0 w1 w2 w3);
-  simpl.  rewrite H0, H1, H2, H3.  tauto.  Qed.
+    We have shown that a substitution is an upper bound if and only if
+    it maps every v to some [quad_term]. If the substitution is to be
+    a supremum as well, the entries in the quad term must themselves
+    be variables. This can be written as [Quad mkV].
 
-(*
+    This holds because any substitution that maps to a quad of
+    variables (for example, [cvquad Vx]) is of the correct form to be
+    an upper bound.
 
+    This is surprisingly difficult to prove. The problem is that we
+    don't immediately get variables in our equations, where we can
+    destruct the terms to see what's going on. To avoid a horrible
+    mess, we use the [term_height] function. The point is that
+    [term_height (quad_term q)] is zero iff [q] only contains
+    variables.
+ *)
 
-Lemma quad_rho_is_vquad {rho q} : subst_sup V F a in_st rho -> (forall
-  v, rho v = quad_term q) -> exists vq, q = vquad_to_quad vq.  Proof.
-  destruct 1 as [ ubH lbH ].  intros qH.  (** The proof starts by
-  picking another upper bound whose terms are simple variables. *) set
-  (x := mkV Vx).  set (qx := vquad_to_quad (mkVQuad Vx Vx Vx Vx)).
-  set (f := (fun v : V => mkF (mkF x x) (mkF x x))).  specialize (lbH
-  f).  assert (ubfH : subst_ub V F a in_st f).  try (apply
-  (@ub_if_form qx f); intro v; destruct v; auto).  specialize (lbH
-  ubfH) as smgH; clear ubfH.  (** The smgH hypothesis says that we can
-  factor [f] through [rho] *) destruct smgH as [ sigma sigmaH ].
+Definition cvquad (v : V) : Quad mkV := mkQuad _ _ v v v v.
+Definition cvquad_subst (v : V) : Subst L := fun v' => quad_term (cvquad v).
 
+Lemma cvquad_is_ub (v : V)
+  : Generality.subst_ub L in_st (cvquad_subst v).
+Proof.
+  set (q := mkQuad _ id (mkV v) (mkV v) (mkV v) (mkV v)).
+  apply (@ub_if_form q).
+  intro v'; auto.
+Qed.
 
+Lemma height_cvquad_subst_v {v v' : V}
+  : term_height (cvquad_subst v v') = 2.
+Proof.
+  apply eq_refl.
+Qed.
 
-  unfold smg in smgH.
+Lemma arity_value (f : Term.F L) : Term.a L f = 2.
+Proof.
+  apply eq_refl.
+Qed.
 
+Lemma height_cvquad_subst_endo {v : V} {t : Term L}
+  : term_height (subst_endo L (cvquad_subst v) t) = 2 + term_height t.
+Proof.
+  revert t; apply Term_ind'; auto using height_cvquad_subst_v.
+  intros f ts IH.
+  unfold cvquad_subst, subst_endo;
+    fold (subst_endo L); fold (cvquad_subst v).
+  unfold term_height; fold (@term_height L).
+  rewrite PeanoNat.Nat.add_succ_r; apply f_equal.
+  rewrite (vec_max_at_map_equal (g := fun n => 2 + n)); auto; clear IH.
+  revert ts; rewrite arity_value.
+  intros; apply vec_max_at_map_incr.
+  intros; repeat (apply le_n_S); assumption.
+Qed.
 
+Lemma height_mkF {t t'}
+  : term_height (mkF t t') = S (max (term_height t) (term_height t')).
+Proof.
+  unfold mkF.
+  unfold term_height at 1; fold (@term_height L).
+  apply f_equal.
+  rewrite (vec_max_at_cons (n := 1)).
+  rewrite (vec_max_at_cons_nil).
+  exact eq_refl.
+Qed.
 
-Lemma UNUSED_subst_to_var_is_var_subst {rho} : (forall v, exists v',
-  rho v = mkV v') -> (exists rho', forall v, rho v = var_subst_subst a
-  rho' v).  Proof.  intro H.  destruct (H Vx) as [ vx Hx ].  destruct
-  (H Vy) as [ vy Hy ].  destruct (H Vz) as [ vz Hz ].  set (f := (fun
-  v => match v with | Vx => vx | Vy => vy | Vz => vz end)).  exists
-  (exist _ f (fin_domain_implies_fin_mod id f decV fullV)).  intro
-  v. unfold var_subst_subst; simpl; unfold f, compose.  destruct v;
-  tauto.  Qed.
+Lemma max_0_elim {a b}
+  : max a b = 0 -> a = 0 /\ b = 0.
+Proof.
+  destruct a, b; auto.
+  intro sH; rewrite <- PeanoNat.Nat.succ_max_distr in sH.
+  contradiction (PeanoNat.Nat.neq_succ_0 _ sH).
+Qed.
 
-(* This is nonsense. We must show that
+Lemma height_0_term {t}
+  : term_height t = 0 -> exists v, t = mkV v.
+Proof.
+  destruct t.
+  - exists v; auto.
+  - simpl; intro eqH; contradiction (PeanoNat.Nat.neq_succ_0 _ eqH).
+Qed.
 
-     rho v = F (F a b) (F c d)
+Lemma height_2_quad_term {tq : Quad id}
+  : term_height (quad_term tq) = 2 ->
+    exists vq : Quad mkV, quad_term tq = quad_term vq.
+Proof.
+  intro htH.
+  destruct tq as [ t0 t1 t2 t3 ]; unfold quad_term, id in htH.
+  assert ((max (max (term_height t0) (term_height t1))
+               (max (term_height t2) (term_height t3))) = 0) as maxH;
+    [ apply eq_add_S, eq_add_S; revert htH; rewrite !height_mkF; auto | ].
+  destruct (max_0_elim maxH) as [ max01H max23H ]; clear htH maxH.
+  destruct (max_0_elim max01H) as [ max0H max1H ]; clear max01H.
+  destruct (max_0_elim max23H) as [ max2H max3H ]; clear max23H.
+  destruct (height_0_term max0H) as [ v0 H0 ]; clear max0H.
+  destruct (height_0_term max1H) as [ v1 H1 ]; clear max1H.
+  destruct (height_0_term max2H) as [ v2 H2 ]; clear max2H.
+  destruct (height_0_term max3H) as [ v3 H3 ]; clear max3H.
+  exists (mkQuad _ mkV v0 v1 v2 v3).
+  unfold quad_term, id; rewrite H0, H1, H2, H3.
+  exact eq_refl.
+Qed.
 
-  where a, b, c, d are disjoint variables. *)
+Lemma height_quad_term {A} {f : A -> Term L} {q : Quad f}
+  : 2 <= term_height (quad_term q).
+Proof.
+  destruct q; unfold quad_term.
+  rewrite !height_mkF; simpl.
+  auto using le_n_S, le_0_n.
+Qed.
 
-Lemma sup_is_var_subst {rho} : subst_sup V F a in_st rho -> exists
-  rho' : var_subst V, forall v, rho v = var_subst_subst a rho' v.
-  Proof.  destruct 1 as [ ubH lbH ].  apply subst_to_var_is_var_subst.
-  (* Unpack form_if_ub to get the general shape of rho *) destruct
-  (form_if_ub ubH) as [ t0 ubH' ]; clear ubH.  destruct ubH' as [ t1
-  ubH ]; destruct ubH as [ t2 ubH ]; destruct ubH as [ t3 ubH ].  (*
-  Now we need to use the fact that rho is a minimal upper bound. *)
-  intro v.  specialize (ubH v).
+Lemma comp_subst_quad_to_var {s0 s1 : Subst L} {v v' : V} {tq : Quad id}
+  : s0 v' = quad_term tq ->
+    comp_subst s1 s0 v' = cvquad_subst v v' ->
+    exists vq : Quad mkV, s0 v' = quad_term vq.
+Proof.
+  intros tqH eqH.
+  rewrite tqH; apply height_2_quad_term.
+  apply PeanoNat.Nat.le_antisymm; [ | exact height_quad_term ].
+  rewrite <- tqH.
+  assert (term_height (comp_subst s1 s0 v') = 2) as heightH;
+    [ exact (f_equal term_height eqH) | ].
+  rewrite <- heightH; exact term_height_comp_subst.
+Qed.
 
-  specialize (ubH Vx).  set (x := mkV Vx).  set (f := (fun v : V =>
-  mkF (mkF x x) (mkF x x))).  specialize (lbH f).  assert (ubfH :
-  subst_ub V F a in_st f); try (apply (@ub_if_form x x x x f); intro
-  v; destruct v; auto).  specialize (lbH ubfH).  destruct lbH as [ f'
-  f'H ].  specialize (f'H Vx).  unfold comp_subst, compose, f in f'H.
-  simpl in f'H.  rewrite ubH in f'H; unfold x in f'H.  injection f'H.
-
-    Check ub_if_form f.  unfold subst_lb in lbH.
-      
-*)
-*)
+Lemma form_if_sup {rho}
+  : Generality.subst_sup L in_st rho ->
+    exists q : Quad mkV, forall v, rho v = quad_term q.
+Proof.
+  destruct 1 as [ ubH lbH ].
+  destruct (form_if_ub ubH) as [ tq tqH ]; clear ubH.
+  destruct (lbH _ (cvquad_is_ub Vx)) as [ rho' rho'H ]; clear lbH.
+  destruct (comp_subst_quad_to_var (tqH Vx) (rho'H Vx)) as [ q qH ].
+  exists q; congruence.
+Qed.
